src/unitb/scheduling/finite.lean
@@ -7,10 +7,13 @@ import unitb.logic
 import unitb.scheduling.basic
 import unitb.models.simple
 
+import data.set.basic
+
+local attribute [-simp] or.comm or.left_comm or.assoc and.comm and.left_comm and.assoc
+
 namespace scheduling.finite
 
-open nat simple function
-
+open nat simple function predicate temporal set
 @[reducible]
 def rrobin (lbl : Type) [pos_finite lbl] : Type :=
 bijection (fin $ succ $ pos_finite.pred_count lbl) lbl
@@ -36,7 +39,7 @@ queue.f (first r queue)
 structure sch_state : Type :=
   (target : t.σ)
   (queue : rrobin lbl)
-  (inv : sch.current (t.req target) queue ∈ t.req target)
+  (inv : sch.current (t.req.apply target) queue ∈ t.req.apply target)
 
 lemma first_mem {req : set lbl}
   (l : rrobin lbl)
@@ -58,7 +61,7 @@ l ∘ (perm.rotate_right (first req l)).rev
 lemma sch.select_inv
   (s : t.σ)
   (q : rrobin lbl)
-: sch.current (t.req s) q ∈ t.req s :=
+: sch.current (t.req.apply s) q ∈ t.req.apply s :=
 begin
   unfold select sch.current,
   apply first_mem _ (t.req_nemp s),
@@ -71,10 +74,13 @@ def sch.first : sch_state :=
 
 noncomputable def sch.step : sch_state → sch_state
  | (sch_state.mk target queue P) :=
-     { target := t.next (sch.current (t.req target) queue) target P
-     , queue := select (t.req target) queue
+     { target := t.next (sch.current (t.req.apply target) queue) target P
+     , queue := select (t.req.apply target) queue
      , inv := sch.select_inv _ _
      }
+
+def sch.is_step : sch_state → sch_state → Prop
+ | s s' := s' = sch.step s
 
 noncomputable def scheduler : program sch_state :=
   { first := sch.first
@@ -82,124 +88,161 @@ noncomputable def scheduler : program sch_state :=
 
 open sch_state unitb subtype has_mem classical
 
-def req (s : sch_state) : set lbl :=
-t.req s.target
+def req : var sch_state (set lbl) :=
+t.req ∘' (sch_state.target : var sch_state t.σ)
 
-noncomputable def next (s : sch_state) : lbl :=
-sch.current (req s) s.queue
+noncomputable def current  : var sch_state lbl :=
+sch.current <$> req <*> queue
 
-def rank (l : lbl) (s : sch_state) : ℕ := (s.queue.g l).val
+def rank (l : lbl) : var (sch_state) ℕ :=
+↑ λ s : sch_state, (s.queue.g l).val
 
-lemma eq_next_or_rank_eq_or_rank_lt {s : sch_state} {l : lbl} (v : ℕ)
-  (h : v = (s.queue.g l).val)
-: l = next s ∨
-  ( l ∉ req s ∧ rank l (sch.step s) = v ) ∨
-  rank l (sch.step s) < v :=
+open scheduling scheduling.unitb
+
+variable (s : sch_state)
+section eq_next_or_rank_eq_or_rank_lt_aux
+variable {v : ℕ}
+variable {l : lbl}
+variable h : (rank l).apply s = v
+include h
+
+section left
+variable Hlt : s.queue.g l < first (req.apply s) s.queue
+include Hlt
+
+private lemma not_requested : l ∉ req.apply s :=
 begin
-  dunfold sch.current select sch.step rank next sch_state.queue sch_state.target req,
-  let target'  := (sch.step _ s).target,
-  let queue' := (sch.step _ s).queue,
   cases s,
-  dunfold sch.step sch_state.queue sch_state.target,
-  cases classical.em (queue.g l = first (t.req target) queue) with Heq Hne,
-  { left,
-    symmetry,
-    rw [bijection.inverse],
+  simp [select,comp,sch.step,sch_state.queue,req,rank] at *,
+  intro h₀,
+  have h₁ : queue.g l ∈ { x | queue.f x ∈ t.req.apply target },
+  { rw [mem_set_of,bijection.g_inv],
+    apply h₀ },
+  have h₂ := minimum_le h₁,
+  apply not_le_of_gt Hlt h₂,
+end
+
+private lemma rank_stable : (rank l).apply (sch.step s) = v :=
+begin
+  cases s,
+  simp [select,comp,sch.step,sch_state.queue,req,rank] at *,
+  rw [comp_g], unfold comp,
+  rw [rev_g ,perm.rotate_right_f_gt_eq_self _ _ Hlt,h] ,
+end
+
+end left
+section right
+
+variable Hgt : s.queue.g l > first (req.apply s) s.queue
+include Hgt
+private lemma rank_dec : (rank l).apply (sch.step s) < v :=
+begin
+  cases s,
+  simp [rank,sch.step,select,req] at *,
+  rw [comp_g], unfold comp,
+  rw [rev_g,perm.rotate_right_f_lt_shifted _ _ Hgt,fin.pred_def,← h],
+  apply pred_lt_self_of_pos,
+  unfold gt at Hgt,
+  rw [fin.lt_def] at Hgt,
+  apply lt_of_le_of_lt _ Hgt,
+  apply zero_le
+end
+end right
+
+end eq_next_or_rank_eq_or_rank_lt_aux
+
+lemma eq_next_or_rank_eq_or_rank_lt  {l : lbl} (v : ℕ)
+  (h : s ⊨ rank l ≃ v)
+: s ⊨ current ≃ ↑l ∨
+      ( s ⊨ - (↑l ∊ req) ∧ sch.step s ⊨ rank l ≃ v ) ∨ sch.step s ⊨ rank l ≺ v :=
+begin
+  -- lifted_pred [temporal.init,sch.is_step] using Hstep h,
+  -- rw Hstep, clear Hstep,
+  -- revert h, generalize : x 0 = s, intro,
+  cases classical.em (s.queue.g l = first ((req t).apply s) s.queue) with Heq Hne,
+  { left, cases s,
+    simp [sch.step,sch_state.queue,sch_state.target,rank,current,req,comp,sch.current] at h ⊢,
+    simp [req] at Heq,
+    rw bijection.inverse,
     symmetry, apply Heq, },
-  cases lt_or_gt_of_ne Hne with Hlt Hgt
-  ; clear Hne,
-  { right,left,
-    split,
-    { intro h₀,
-      have h₁ : queue.g l ∈ { x | queue.f x ∈ t.req target },
-      { rw [mem_set_of,bijection.g_inv],
-        apply h₀ },
-      have h₂ := minimum_le h₁,
-      apply not_le_of_gt Hlt h₂, },
-    { dunfold select comp sch.step sch_state.queue,
-      rw [comp_g], unfold comp,
-      rw [rev_g ,h,perm.rotate_right_f_gt_eq_self _ _ Hlt], } },
-  { right,right,
-    unfold comp select,
-    rw [comp_g], unfold comp,
-    rw [rev_g,perm.rotate_right_f_lt_shifted _ _ Hgt,fin.pred_def,← h],
-    apply pred_lt_self_of_pos,
-    unfold gt at Hgt,
-    rw [fin.lt_def,← h] at Hgt,
-    apply lt_of_le_of_lt _ Hgt,
-    apply zero_le },
+  cases lt_or_gt_of_ne Hne with Hlt Hgt ; clear Hne,
+  { right, left, split, simp,
+    apply not_requested t s ; assumption ,
+    apply rank_stable t s ; assumption },
+  { right, right,
+    apply rank_dec t s ; assumption , },
 end
 
 lemma fair_schedule_step  (l : lbl) (v : ℕ)
-:  mem l ∘ req ⋀ (eq v ∘ rank l) ↦ (flip has_lt.lt v ∘ rank l) ⋁ eq l ∘ next in scheduler :=
+:  ↑l ∊ req ⋀ rank l ≃ v ↦ rank l ≺ v ⋁ current ≃ l in scheduler :=
 begin
   unfold scheduler,
   apply leads_to_step,
   intros σ Heq Hnnext,
-  simp, simp at Heq,
-  unfold function.comp flip sch.step, -- next rank subtype.val,
-  cases Heq with Heq Hmem,
-  have HH := eq_next_or_rank_eq_or_rank_lt _ v Heq,
+  -- simp, simp at Heq Hnnext,
+  -- unfold rank function.comp flip sch.step, -- next rank subtype.val,
+  cases Heq with Hmem Heq,
+  have HH := eq_next_or_rank_eq_or_rank_lt _ _ v Heq,
   rw or_iff_not_imp at HH,
-  simp [not_or_iff_not_and_not] at Hnnext,
-  have HH' := HH Hnnext.left,
+  simp [not_or_iff_not_and_not] at Hnnext HH,
+  have HH' := HH Hnnext.right,
   rw [or_iff_not_imp,not_and_iff_not_or_not,not_not_iff_self] at HH',
-  right, apply HH', clear HH' HH,
-  apply or.intro_left _ Hmem,
+  left, apply HH', clear HH' HH,
+  left, simp at Hmem, assumption
 end
 
 lemma stable_queue_ranking (l : lbl) (v : ℕ)
-: unless scheduler (eq v ∘ rank l) (flip has_lt.lt v ∘ rank l ⋁ eq l ∘ next) :=
+: unless scheduler (rank l ≃ v) (rank l ≺ v ⋁ current ≃ l) :=
 begin
   unfold scheduler,
   apply unless_step,
   intros σ Heq Hnnext,
   simp,
   simp [not_or_iff_not_and_not] at Hnnext,
-  unfold function.comp,
-  unfold comp at Heq,
-  apply or.imp _ _ (eq_next_or_rank_eq_or_rank_lt _ _ Heq),
-  { intro h, cases Hnnext.left h, },
-  { apply or.imp_left,
-    intro h, cases h with _ h, rw h, },
+  have := eq_next_or_rank_eq_or_rank_lt _ _ _ Heq, revert this,
+  simp, monotonicity, intro h,
+  cases h with h h,
+  { cases Hnnext.right h, },
+  { left, rw [h.right], },
 end
 
 lemma INIT
-: system.init scheduler (eq t.s₀ ∘ sch_state.target) :=
+: system.init scheduler (↑sch_state.target ≃ (t.s₀ : var sch_state t.σ)) :=
 begin
-  unfold system.init program.init function.comp scheduler,
+  simp [system.init,program.init,scheduler],
   refl,
 end
 
 lemma STEP
 : co' scheduler
     (λ (σ σ' : sch_state),
-       ∃ P, σ'.target = t.next (next σ) σ.target P) :=
+       ∃ P, σ'.target = t.next (current.apply σ) σ.target P) :=
 begin
   unfold co',
   intros σ σ',
-  unfold step has_safety.step is_step,
+  dunfold step has_safety.step is_step,
   intros H,
-  existsi σ.inv,
+  have P : (current t).apply σ ∈ (t.req).apply (σ.target),
+  { simp [current,req], exact σ.inv,  },
+  existsi P,
   rw H,
   unfold function.comp scheduler program.step subtype.val sch.step,
   cases σ,
-  dunfold sch.step sch_state.target,
-  refl,
+  simp [sch.step,sch_state.target,current,req],
 end
 
-lemma INV (σ : sch_state)
-: next σ ∈ t.req (σ.target) :=
-σ.inv
+lemma INV
+: ∀ σ, σ ⊨ current ∊ t.req ∘' sch_state.target :=
+by { assume σ, simp [current,req], apply σ.inv, }
 
-lemma PROG (l)
+lemma PROG (l : lbl)
 : often_imp_often scheduler
-      (mem l ∘ t.req ∘ sch_state.target)
-      (eq l ∘ next) :=
+      (↑l ∊ req)
+      (current ≃ l) :=
 begin
-  apply often_imp_often.induct _ _ _ nat.lt_wf,
+  apply often_imp_often.induct ℕ _ _ ,
+  apply stable_queue_ranking _ l,
   apply fair_schedule_step _ l,
-  apply stable_queue_ranking _ l
 end
 
 end
@@ -215,7 +258,7 @@ noncomputable def scheduler_spec
   { s := program $ @sch_state lbl _ r
   , sem := _
   , F := @scheduler _ _ _
-  , ch := next r
+  , ch := current r
   , object := _
   , INIT := INIT r
   , STEP := STEP r
@@ -234,7 +277,6 @@ begin
   have h : pos_finite lbl,
   { apply pos_of_finite ; apply_instance },
   apply unitb.scheduling r (scheduling.finite.scheduler_spec r),
-  apply_instance
 end
 
 end scheduling.finite
